thys/MSO_Regex_Equivalence/M2L_Equivalence_Checking.thy
@@ -10,18 +10,16 @@ imports
   Init_Normalization
   M2L_Normalization
   Pi_Regular_Exp_Dual
+  "~~/src/Tools/Permanent_Interpretation"
 begin
 (*>*)
 
-type_synonym 'a T = "'a atom"
-
-definition [code del]: "\<DD> \<equiv> \<lambda>(\<Sigma>::'a::linorder list). embed.lderiv lookup (\<epsilon> \<Sigma>)"
-definition [code del]: "Co\<DD> \<equiv> \<lambda>(\<Sigma>::'a::linorder list). embed.lderiv_dual lookup (\<epsilon> \<Sigma>)"
-
-interpretation embed "set o \<sigma> \<Sigma>" "wf_atom \<Sigma>" \<pi> lookup "\<epsilon> \<Sigma>" for \<Sigma> :: "'a :: linorder list"
-  where "embed.lderiv lookup (\<epsilon> \<Sigma>) = \<DD> \<Sigma>"
-    and "embed.lderiv_dual lookup (\<epsilon> \<Sigma>) = Co\<DD> \<Sigma>"
-  by unfold_locales (auto simp: \<sigma>_def \<pi>_def \<epsilon>_def \<DD>_def Co\<DD>_def)
+permanent_interpretation embed "set o \<sigma> \<Sigma>" "wf_atom \<Sigma>" \<pi> lookup "\<epsilon> \<Sigma>"
+  for \<Sigma> :: "'a :: linorder list"
+  defining
+      \<DD> = "embed.lderiv lookup (\<epsilon> \<Sigma>)"
+  and Co\<DD> = "embed.lderiv_dual lookup (\<epsilon> \<Sigma>)"
+  by unfold_locales (auto simp: \<sigma>_def \<pi>_def \<epsilon>_def set_n_lists)
 
 lemma enum_not_empty[simp]: "Enum.enum \<noteq> []" (is "?enum \<noteq> []")
 proof (rule notI)
@@ -30,35 +28,19 @@ proof (rule notI)
   thus False unfolding UNIV_enum[symmetric] by simp
 qed
 
-definition pre_wf_formula where [code del]:
-  "pre_wf_formula \<equiv> formula.pre_wf_formula Enum.enum"
-definition wf_formula where [code del]:
-  "wf_formula \<equiv> formula.wf_formula Enum.enum"
-definition valid_ENC where [code del]: "valid_ENC \<equiv> formula.valid_ENC"
-definition ENC where [code del]: "ENC \<equiv> formula.ENC"
-definition dec_interp where [code del]: "dec_interp \<equiv> formula.dec_interp"
-definition rexp_of where [code del]: "rexp_of \<equiv> formula.rexp_of"
-definition rexp_of_alt where [code del]: "rexp_of_alt \<equiv> formula.rexp_of_alt"
-definition rexp_of_alt' where [code del]: "rexp_of_alt' \<equiv> formula.rexp_of_alt'"
-definition rexp_of' where [code del]: "rexp_of' \<equiv> formula.rexp_of'"
-definition rexp_of'' where [code del]: "rexp_of'' \<equiv> formula.rexp_of''"
-
-lemmas formula_defs = pre_wf_formula_def wf_formula_def
-  rexp_of_def rexp_of'_def rexp_of''_def rexp_of_alt_def rexp_of_alt'_def
-  ENC_def dec_interp_def valid_ENC_def FOV_def SOV_def
-
-interpretation \<Phi>: formula "Enum.enum :: 'a :: {enum, linorder} list"
-  where "\<Phi>.pre_wf_formula = pre_wf_formula"
-  and   "\<Phi>.wf_formula = wf_formula"
-  and   "\<Phi>.rexp_of = rexp_of"
-  and   "\<Phi>.rexp_of_alt = rexp_of_alt"
-  and   "\<Phi>.rexp_of_alt' = rexp_of_alt'"
-  and   "\<Phi>.rexp_of' = rexp_of'"
-  and   "\<Phi>.rexp_of'' = rexp_of''"
-  and   "\<Phi>.valid_ENC = valid_ENC"
-  and   "\<Phi>.ENC = ENC"
-  and   "\<Phi>.dec_interp = dec_interp"
-  by unfold_locales (auto simp: \<sigma>_def \<pi>_def formula_defs set_n_lists)
+permanent_interpretation \<Phi>: formula "Enum.enum :: 'a :: {enum, linorder} list"
+  defining
+      pre_wf_formula = \<Phi>.pre_wf_formula
+  and wf_formula = \<Phi>.wf_formula
+  and rexp_of = \<Phi>.rexp_of
+  and rexp_of_alt = \<Phi>.rexp_of_alt
+  and rexp_of_alt' = \<Phi>.rexp_of_alt'
+  and rexp_of' = \<Phi>.rexp_of'
+  and rexp_of'' = \<Phi>.rexp_of''
+  and valid_ENC = \<Phi>.valid_ENC
+  and ENC = \<Phi>.ENC
+  and dec_interp = \<Phi>.dec_interp
+  by unfold_locales (auto simp: \<sigma>_def \<pi>_def set_n_lists)
 
 lemma lang_Plus_Zero: "lang \<Sigma> n (Plus r One) = lang \<Sigma> n (Plus s One) \<longleftrightarrow> lang \<Sigma> n r - {[]} = lang \<Sigma> n s - {[]}"
   by auto
@@ -69,38 +51,24 @@ lemmas lang\<^sub>M\<^sub>2\<^sub>L_rexp_of''_norm = trans[OF sym[OF \<Phi>.lang
 
 setup {* Sign.map_naming (Name_Space.mandatory_path "slow") *}
 
-definition [code del]: "test \<equiv> rexp_DA.test (final :: 'a :: linorder atom rexp \<Rightarrow> bool)"
-definition [code del]: "step \<equiv> \<lambda>(\<Sigma>::'a::linorder list). rexp_DA.step (\<sigma> \<Sigma>) (\<lambda>a r. \<guillemotleft>\<DD> \<Sigma> a r\<guillemotright>) pnorm"
-definition [code del]: "closure \<equiv> \<lambda>(\<Sigma>::'a::linorder list). rexp_DA.closure (\<sigma> \<Sigma>) (\<lambda>a r. \<guillemotleft>\<DD> \<Sigma> a r\<guillemotright>) final pnorm"
-definition [code del]: "check_eqvRE \<equiv> \<lambda>(\<Sigma>::'a::linorder list). rexp_DA.check_eqv (\<sigma> \<Sigma>) (\<lambda>x. \<guillemotleft>pnorm (inorm x)\<guillemotright>) (\<lambda>a r. \<guillemotleft>\<DD> \<Sigma> a r\<guillemotright>) final pnorm"
-definition test_invariant  :: "(('a::linorder \<times> bool list) list \<times> _) list \<times> _ \<Rightarrow> _" where
-  [code del]: "test_invariant \<equiv> rexp_DA.test_invariant (final :: 'a atom rexp \<Rightarrow> bool)"
-definition [code del]: "step_invariant \<equiv> \<lambda>(\<Sigma>::'a::linorder list). rexp_DA.step_invariant (\<sigma> \<Sigma>) (\<lambda>a r. \<guillemotleft>\<DD> \<Sigma> a r\<guillemotright>) pnorm"
-definition [code del]: "closure_invariant \<equiv> \<lambda>(\<Sigma>::'a::linorder list). rexp_DA.closure_invariant (\<sigma> \<Sigma>) (\<lambda>a r. \<guillemotleft>\<DD> \<Sigma> a r\<guillemotright>) final pnorm"
-definition [code del]: "counterexampleRE \<equiv> \<lambda>(\<Sigma>::'a::linorder list). rexp_DA.counterexample (\<sigma> \<Sigma>) (\<lambda>x. \<guillemotleft>pnorm (inorm x)\<guillemotright>) (\<lambda>a r. \<guillemotleft>\<DD> \<Sigma> a r\<guillemotright>) final pnorm"
-definition [code del]: "reachable \<equiv> \<lambda>(\<Sigma>::'a::linorder list). rexp_DA.reachable (\<sigma> \<Sigma>) (\<lambda>x. \<guillemotleft>pnorm (inorm x)\<guillemotright>) (\<lambda>a r. \<guillemotleft>\<DD> \<Sigma> a r\<guillemotright>) pnorm"
-definition [code del]: "automaton \<equiv> \<lambda>(\<Sigma>::'a::linorder list). rexp_DA.automaton (\<sigma> \<Sigma>) (\<lambda>x. \<guillemotleft>pnorm (inorm x)\<guillemotright>) (\<lambda>a r. \<guillemotleft>\<DD> \<Sigma> a r\<guillemotright>) pnorm"
-
-lemmas rexp_DFA_defs = slow.test_invariant_def slow.test_def slow.step_invariant_def slow.step_def
-  slow.closure_invariant_def slow.closure_def slow.check_eqvRE_def slow.counterexampleRE_def
-  slow.reachable_def slow.automaton_def
-
-interpretation D: rexp_DFA "\<sigma> \<Sigma>" "wf_atom \<Sigma>" \<pi> lookup "\<lambda>x. \<guillemotleft>pnorm (inorm x)\<guillemotright>"
+permanent_interpretation D: rexp_DFA "\<sigma> \<Sigma>" "wf_atom \<Sigma>" \<pi> lookup "\<lambda>x. \<guillemotleft>pnorm (inorm x)\<guillemotright>"
   "\<lambda>a r. \<guillemotleft>\<DD> \<Sigma> a r\<guillemotright>" final "alphabet.wf (wf_atom \<Sigma>) n" pnorm "lang \<Sigma> n" n
   for \<Sigma> :: "'a :: linorder list" and n :: nat
-  where "rexp_DA.test final = slow.test"
-    and "rexp_DA.step (\<sigma> \<Sigma>) (\<lambda>a r. \<guillemotleft>\<DD> \<Sigma> a r\<guillemotright>) pnorm n = slow.step \<Sigma> n"
-    and "rexp_DA.closure (\<sigma> \<Sigma>) (\<lambda>a r. \<guillemotleft>\<DD> \<Sigma> a r\<guillemotright>) final pnorm n = slow.closure \<Sigma> n"
-    and "rexp_DA.check_eqv (\<sigma> \<Sigma>) (\<lambda>x. \<guillemotleft>pnorm (inorm x)\<guillemotright>) (\<lambda>a r. \<guillemotleft>\<DD> \<Sigma> a r\<guillemotright>) final pnorm n = slow.check_eqvRE \<Sigma> n"
-    and "rexp_DA.test_invariant final = slow.test_invariant"
-    and "rexp_DA.step_invariant (\<sigma> \<Sigma>) (\<lambda>a r. \<guillemotleft>\<DD> \<Sigma> a r\<guillemotright>) pnorm n = slow.step_invariant \<Sigma> n"
-    and "rexp_DA.closure_invariant (\<sigma> \<Sigma>) (\<lambda>a r. \<guillemotleft>\<DD> \<Sigma> a r\<guillemotright>) final pnorm n = slow.closure_invariant \<Sigma> n"
-    and "rexp_DA.counterexample (\<sigma> \<Sigma>) (\<lambda>x. \<guillemotleft>pnorm (inorm x)\<guillemotright>) (\<lambda>a r. \<guillemotleft>\<DD> \<Sigma> a r\<guillemotright>) final pnorm n = slow.counterexampleRE \<Sigma> n"
-    and "rexp_DA.reachable (\<sigma> \<Sigma>) (\<lambda>x. \<guillemotleft>pnorm (inorm x)\<guillemotright>) (\<lambda>a r. \<guillemotleft>\<DD> \<Sigma> a r\<guillemotright>) pnorm n = slow.reachable \<Sigma> n"
-    and "rexp_DA.automaton (\<sigma> \<Sigma>) (\<lambda>x. \<guillemotleft>pnorm (inorm x)\<guillemotright>) (\<lambda>a r. \<guillemotleft>\<DD> \<Sigma> a r\<guillemotright>) pnorm n = slow.automaton \<Sigma> n"
-    by unfold_locales (auto simp only: comp_apply
-      ACI_norm_wf ACI_norm_lang wf_inorm lang_inorm wf_pnorm lang_pnorm wf_lderiv lang_lderiv
-      lang_final finite_fold_lderiv slow.rexp_DFA_defs dest!: lang_subset_lists)
+  defining
+      test = "rexp_DA.test (final :: 'a atom rexp \<Rightarrow> bool)"
+  and step = "rexp_DA.step (\<sigma> \<Sigma>) (\<lambda>a r. \<guillemotleft>\<DD> \<Sigma> a r\<guillemotright>) pnorm n"
+  and closure = "rexp_DA.closure (\<sigma> \<Sigma>) (\<lambda>a r. \<guillemotleft>\<DD> \<Sigma> a r\<guillemotright>) final pnorm n"
+  and check_eqvRE = "rexp_DA.check_eqv (\<sigma> \<Sigma>) (\<lambda>x. \<guillemotleft>pnorm (inorm x)\<guillemotright>) (\<lambda>a r. \<guillemotleft>\<DD> \<Sigma> a r\<guillemotright>) final pnorm n"
+  and test_invariant = "rexp_DA.test_invariant (final :: 'a atom rexp \<Rightarrow> bool) ::
+    (('a \<times> bool list) list \<times> _) list \<times> _ \<Rightarrow> bool"
+  and step_invariant = "rexp_DA.step_invariant (\<sigma> \<Sigma>) (\<lambda>a r. \<guillemotleft>\<DD> \<Sigma> a r\<guillemotright>) pnorm n"
+  and closure_invariant = "rexp_DA.closure_invariant (\<sigma> \<Sigma>) (\<lambda>a r. \<guillemotleft>\<DD> \<Sigma> a r\<guillemotright>) final pnorm n"
+  and counterexampleRE = "rexp_DA.counterexample (\<sigma> \<Sigma>) (\<lambda>x. \<guillemotleft>pnorm (inorm x)\<guillemotright>) (\<lambda>a r. \<guillemotleft>\<DD> \<Sigma> a r\<guillemotright>) final pnorm n"
+  and reachable = "rexp_DA.reachable (\<sigma> \<Sigma>) (\<lambda>x. \<guillemotleft>pnorm (inorm x)\<guillemotright>) (\<lambda>a r. \<guillemotleft>\<DD> \<Sigma> a r\<guillemotright>) pnorm n"
+  and automaton = "rexp_DA.automaton (\<sigma> \<Sigma>) (\<lambda>x. \<guillemotleft>pnorm (inorm x)\<guillemotright>) (\<lambda>a r. \<guillemotleft>\<DD> \<Sigma> a r\<guillemotright>) pnorm n"
+  by unfold_locales (auto simp only: comp_apply
+    ACI_norm_wf ACI_norm_lang wf_inorm lang_inorm wf_pnorm lang_pnorm wf_lderiv lang_lderiv
+    lang_final finite_fold_lderiv dest!: lang_subset_lists)
 
 definition check_eqv where
 "check_eqv n \<phi> \<psi> \<longleftrightarrow> wf_formula n (FOr \<phi> \<psi>) \<and>
@@ -128,39 +96,25 @@ setup {* Sign.map_naming Name_Space.parent_path *}
 
 setup {* Sign.map_naming (Name_Space.mandatory_path "fast") *}
 
-definition [code del]: "test \<equiv> rexp_DA.test (final :: 'a :: linorder atom rexp \<Rightarrow> bool)"
-definition [code del]: "step \<equiv> \<lambda>(\<Sigma>::'a::linorder list). rexp_DA.step (\<sigma> \<Sigma>) (\<lambda>a r. pnorm (\<DD> \<Sigma> a r)) id"
-definition [code del]: "closure \<equiv> \<lambda>(\<Sigma>::'a::linorder list). rexp_DA.closure (\<sigma> \<Sigma>) (\<lambda>a r. pnorm (\<DD> \<Sigma> a r)) final id"
-definition [code del]: "check_eqvRE \<equiv> \<lambda>(\<Sigma>::'a::linorder list). rexp_DA.check_eqv (\<sigma> \<Sigma>) (\<lambda>x. pnorm (inorm x)) (\<lambda>a r. pnorm (\<DD> \<Sigma> a r)) final id"
-definition test_invariant  :: "(('a::linorder \<times> bool list) list \<times> _) list \<times> _ \<Rightarrow> _" where
-  [code del]: "test_invariant \<equiv> rexp_DA.test_invariant (final :: 'a atom rexp \<Rightarrow> bool)"
-definition [code del]: "step_invariant \<equiv> \<lambda>(\<Sigma>::'a::linorder list). rexp_DA.step_invariant (\<sigma> \<Sigma>) (\<lambda>a r. pnorm (\<DD> \<Sigma> a r)) id"
-definition [code del]: "closure_invariant \<equiv> \<lambda>(\<Sigma>::'a::linorder list). rexp_DA.closure_invariant (\<sigma> \<Sigma>) (\<lambda>a r. pnorm (\<DD> \<Sigma> a r)) final id"
-definition [code del]: "counterexampleRE \<equiv> \<lambda>(\<Sigma>::'a::linorder list). rexp_DA.counterexample (\<sigma> \<Sigma>) (\<lambda>x. pnorm (inorm x)) (\<lambda>a r. pnorm (\<DD> \<Sigma> a r)) final id"
-definition [code del]: "reachable \<equiv> \<lambda>(\<Sigma>::'a::linorder list). rexp_DA.reachable (\<sigma> \<Sigma>) (\<lambda>x. pnorm (inorm x)) (\<lambda>a r. pnorm (\<DD> \<Sigma> a r)) id"
-definition [code del]: "automaton \<equiv> \<lambda>(\<Sigma>::'a::linorder list). rexp_DA.automaton (\<sigma> \<Sigma>) (\<lambda>x. pnorm (inorm x)) (\<lambda>a r. pnorm (\<DD> \<Sigma> a r)) id"
-
-lemmas rexp_DFA_defs = fast.test_invariant_def fast.test_def fast.step_invariant_def fast.step_def
-  fast.closure_invariant_def fast.closure_def fast.check_eqvRE_def fast.counterexampleRE_def
-  fast.reachable_def fast.automaton_def
-
-interpretation D: rexp_DA_no_post "\<sigma> \<Sigma>" "wf_atom \<Sigma>" \<pi> lookup "\<lambda>x. pnorm (inorm x)"
+permanent_interpretation D: rexp_DA_no_post "\<sigma> \<Sigma>" "wf_atom \<Sigma>" \<pi> lookup "\<lambda>x. pnorm (inorm x)"
   "\<lambda>a r. pnorm (\<DD> \<Sigma> a r)" final "alphabet.wf (wf_atom \<Sigma>) n" "lang \<Sigma> n" n
   for \<Sigma> :: "'a :: linorder list" and n :: nat
-  where "rexp_DA.test final = fast.test"
-    and "rexp_DA.step (\<sigma> \<Sigma>) (\<lambda>a r. pnorm (\<DD> \<Sigma> a r)) id n = fast.step \<Sigma> n"
-    and "rexp_DA.closure (\<sigma> \<Sigma>) (\<lambda>a r. pnorm (\<DD> \<Sigma> a r)) final id n = fast.closure \<Sigma> n"
-    and "rexp_DA.check_eqv (\<sigma> \<Sigma>) (\<lambda>x. pnorm (inorm x)) (\<lambda>a r. pnorm (\<DD> \<Sigma> a r)) final id n = fast.check_eqvRE \<Sigma> n"
-    and "rexp_DA.test_invariant final = fast.test_invariant"
-    and "rexp_DA.step_invariant (\<sigma> \<Sigma>) (\<lambda>a r. pnorm (\<DD> \<Sigma> a r)) id n = fast.step_invariant \<Sigma> n"
-    and "rexp_DA.closure_invariant (\<sigma> \<Sigma>) (\<lambda>a r. pnorm (\<DD> \<Sigma> a r)) final id n = fast.closure_invariant \<Sigma> n"
-    and "rexp_DA.counterexample (\<sigma> \<Sigma>) (\<lambda>x. pnorm (inorm x)) (\<lambda>a r. pnorm (\<DD> \<Sigma> a r)) final id n = fast.counterexampleRE \<Sigma> n"
-    and "rexp_DA.reachable (\<sigma> \<Sigma>) (\<lambda>x. pnorm (inorm x)) (\<lambda>a r. pnorm (\<DD> \<Sigma> a r)) id n = fast.reachable \<Sigma> n"
-    and "rexp_DA.automaton (\<sigma> \<Sigma>) (\<lambda>x. pnorm (inorm x)) (\<lambda>a r. pnorm (\<DD> \<Sigma> a r)) id n = fast.automaton \<Sigma> n"
-    by unfold_locales (auto simp only: comp_apply
-      ACI_norm_wf ACI_norm_lang wf_inorm lang_inorm wf_pnorm lang_pnorm wf_lderiv lang_lderiv id_apply
-      lang_final fast.rexp_DFA_defs dest!: lang_subset_lists)
-export_code fast.step in SML
+  defining
+      test = "rexp_DA.test (final :: 'a atom rexp \<Rightarrow> bool)"
+  and step = "rexp_DA.step (\<sigma> \<Sigma>) (\<lambda>a r. pnorm (\<DD> \<Sigma> a r)) id n"
+  and closure = "rexp_DA.closure (\<sigma> \<Sigma>) (\<lambda>a r. pnorm (\<DD> \<Sigma> a r)) final id n"
+  and check_eqvRE = "rexp_DA.check_eqv (\<sigma> \<Sigma>) (\<lambda>x. pnorm (inorm x)) (\<lambda>a r. pnorm (\<DD> \<Sigma> a r)) final id n"
+  and test_invariant = "rexp_DA.test_invariant (final :: 'a atom rexp \<Rightarrow> bool) ::
+    (('a \<times> bool list) list \<times> _) list \<times> _ \<Rightarrow> bool"
+  and step_invariant = "rexp_DA.step_invariant (\<sigma> \<Sigma>) (\<lambda>a r. pnorm (\<DD> \<Sigma> a r)) id n"
+  and closure_invariant = "rexp_DA.closure_invariant (\<sigma> \<Sigma>) (\<lambda>a r. pnorm (\<DD> \<Sigma> a r)) final id n"
+  and counterexampleRE = "rexp_DA.counterexample (\<sigma> \<Sigma>) (\<lambda>x. pnorm (inorm x)) (\<lambda>a r. pnorm (\<DD> \<Sigma> a r)) final id n"
+  and reachable = "rexp_DA.reachable (\<sigma> \<Sigma>) (\<lambda>x. pnorm (inorm x)) (\<lambda>a r. pnorm (\<DD> \<Sigma> a r)) id n"
+  and automaton = "rexp_DA.automaton (\<sigma> \<Sigma>) (\<lambda>x. pnorm (inorm x)) (\<lambda>a r. pnorm (\<DD> \<Sigma> a r)) id n"
+  by unfold_locales (auto simp only: comp_apply
+    ACI_norm_wf ACI_norm_lang wf_inorm lang_inorm wf_pnorm lang_pnorm wf_lderiv lang_lderiv id_apply
+    lang_final dest!: lang_subset_lists)
+
 definition check_eqv where
 "check_eqv n \<phi> \<psi> \<longleftrightarrow> wf_formula n (FOr \<phi> \<psi>) \<and>
    fast.check_eqvRE Enum.enum n (Plus (rexp_of'' n (norm \<phi>)) One) (Plus (rexp_of'' n (norm \<psi>)) One)"
@@ -179,41 +133,28 @@ setup {* Sign.map_naming Name_Space.parent_path *}
 
 setup {* Sign.map_naming (Name_Space.mandatory_path "dual") *}
 
-definition [code del]: "test \<equiv> rexp_DA.test (final_dual :: 'a :: linorder atom rexp_dual \<Rightarrow> bool)"
-definition [code del]: "step \<equiv> \<lambda>(\<Sigma>::'a::linorder list). rexp_DA.step (\<sigma> \<Sigma>) (\<lambda>a r. pnorm_dual (Co\<DD> \<Sigma> a r)) id"
-definition [code del]: "closure \<equiv> \<lambda>(\<Sigma>::'a::linorder list). rexp_DA.closure (\<sigma> \<Sigma>) (\<lambda>a r. pnorm_dual (Co\<DD> \<Sigma> a r)) final_dual id"
-definition [code del]: "check_eqvRE \<equiv> \<lambda>(\<Sigma>::'a::linorder list). rexp_DA.check_eqv (\<sigma> \<Sigma>) (\<lambda>x. pnorm_dual (rexp_dual_of (inorm x))) (\<lambda>a r. pnorm_dual (Co\<DD> \<Sigma> a r)) final_dual id"
-definition test_invariant  :: "(('a::linorder \<times> bool list) list \<times> _) list \<times> _ \<Rightarrow> _" where
-  [code del]: "test_invariant \<equiv> rexp_DA.test_invariant (final_dual :: 'a atom rexp_dual \<Rightarrow> bool)"
-definition [code del]: "step_invariant \<equiv> \<lambda>(\<Sigma>::'a::linorder list). rexp_DA.step_invariant (\<sigma> \<Sigma>) (\<lambda>a r. pnorm_dual (Co\<DD> \<Sigma> a r)) id"
-definition [code del]: "closure_invariant \<equiv> \<lambda>(\<Sigma>::'a::linorder list). rexp_DA.closure_invariant (\<sigma> \<Sigma>) (\<lambda>a r. pnorm_dual (Co\<DD> \<Sigma> a r)) final_dual id"
-definition [code del]: "counterexampleRE \<equiv> \<lambda>(\<Sigma>::'a::linorder list). rexp_DA.counterexample (\<sigma> \<Sigma>) (\<lambda>x. pnorm_dual (rexp_dual_of (inorm x))) (\<lambda>a r. pnorm_dual (Co\<DD> \<Sigma> a r)) final_dual id"
-definition [code del]: "reachable \<equiv> \<lambda>(\<Sigma>::'a::linorder list). rexp_DA.reachable (\<sigma> \<Sigma>) (\<lambda>x. pnorm_dual (rexp_dual_of (inorm x))) (\<lambda>a r. pnorm_dual (Co\<DD> \<Sigma> a r)) id"
-definition [code del]: "automaton \<equiv> \<lambda>(\<Sigma>::'a::linorder list). rexp_DA.automaton (\<sigma> \<Sigma>) (\<lambda>x. pnorm_dual (rexp_dual_of (inorm x))) (\<lambda>a r. pnorm_dual (Co\<DD> \<Sigma> a r)) id"
-
-lemmas rexp_dual_DFA_defs = dual.test_invariant_def dual.test_def dual.step_invariant_def dual.step_def
-  dual.closure_invariant_def dual.closure_def dual.check_eqvRE_def dual.counterexampleRE_def
-  dual.reachable_def dual.automaton_def
-
-interpretation D: rexp_DA_no_post "\<sigma> \<Sigma>" "wf_atom \<Sigma>" \<pi> lookup "\<lambda>x. pnorm_dual (rexp_dual_of (inorm x))"
-  "\<lambda>a r. pnorm_dual (Co\<DD> \<Sigma> a r)" final_dual "alphabet.wf_dual (wf_atom \<Sigma>) n" "lang_dual \<Sigma> n" n
+permanent_interpretation D: rexp_DA_no_post "\<sigma> \<Sigma>" "wf_atom \<Sigma>" \<pi> lookup
+  "\<lambda>x. pnorm_dual (rexp_dual_of (inorm x))" "\<lambda>a r. pnorm_dual (Co\<DD> \<Sigma> a r)" final_dual
+  "alphabet.wf_dual (wf_atom \<Sigma>) n" "lang_dual \<Sigma> n" n
   for \<Sigma> :: "'a :: linorder list" and n :: nat
-  where "rexp_DA.test final_dual = dual.test"
-    and "rexp_DA.step (\<sigma> \<Sigma>) (\<lambda>a r. pnorm_dual (Co\<DD> \<Sigma> a r)) id n = dual.step \<Sigma> n"
-    and "rexp_DA.closure (\<sigma> \<Sigma>) (\<lambda>a r. pnorm_dual (Co\<DD> \<Sigma> a r)) final_dual id n = dual.closure \<Sigma> n"
-    and "rexp_DA.check_eqv (\<sigma> \<Sigma>) (\<lambda>x. pnorm_dual (rexp_dual_of (inorm x))) (\<lambda>a r. pnorm_dual (Co\<DD> \<Sigma> a r)) final_dual id n = dual.check_eqvRE \<Sigma> n"
-    and "rexp_DA.test_invariant final_dual = dual.test_invariant"
-    and "rexp_DA.step_invariant (\<sigma> \<Sigma>) (\<lambda>a r. pnorm_dual (Co\<DD> \<Sigma> a r)) id n = dual.step_invariant \<Sigma> n"
-    and "rexp_DA.closure_invariant (\<sigma> \<Sigma>) (\<lambda>a r. pnorm_dual (Co\<DD> \<Sigma> a r)) final_dual id n = dual.closure_invariant \<Sigma> n"
-    and "rexp_DA.counterexample (\<sigma> \<Sigma>) (\<lambda>x. pnorm_dual (rexp_dual_of (inorm x))) (\<lambda>a r. pnorm_dual (Co\<DD> \<Sigma> a r)) final_dual id n = dual.counterexampleRE \<Sigma> n"
-    and "rexp_DA.reachable (\<sigma> \<Sigma>) (\<lambda>x. pnorm_dual (rexp_dual_of (inorm x))) (\<lambda>a r. pnorm_dual (Co\<DD> \<Sigma> a r)) id n = dual.reachable \<Sigma> n"
-    and "rexp_DA.automaton (\<sigma> \<Sigma>) (\<lambda>x. pnorm_dual (rexp_dual_of (inorm x))) (\<lambda>a r. pnorm_dual (Co\<DD> \<Sigma> a r)) id n = dual.automaton \<Sigma> n"
-    by unfold_locales (auto simp only: comp_apply id_apply
-      wf_inorm lang_inorm
-      wf_dual_pnorm_dual lang_dual_pnorm_dual
-      wf_dual_rexp_dual_of lang_dual_rexp_dual_of
-      wf_dual_lderiv_dual lang_dual_lderiv_dual
-      lang_dual_final_dual dual.rexp_dual_DFA_defs dest!: lang_dual_subset_lists)
+  defining
+      test = "rexp_DA.test (final_dual :: 'a atom rexp_dual \<Rightarrow> bool)"
+  and step = "rexp_DA.step (\<sigma> \<Sigma>) (\<lambda>a r. pnorm_dual (Co\<DD> \<Sigma> a r)) id n"
+  and closure = "rexp_DA.closure (\<sigma> \<Sigma>) (\<lambda>a r. pnorm_dual (Co\<DD> \<Sigma> a r)) final_dual id n"
+  and check_eqvRE = "rexp_DA.check_eqv (\<sigma> \<Sigma>) (\<lambda>x. pnorm_dual (rexp_dual_of (inorm x))) (\<lambda>a r. pnorm_dual (Co\<DD> \<Sigma> a r)) final_dual id n"
+  and test_invariant = "rexp_DA.test_invariant (final_dual :: 'a atom rexp_dual \<Rightarrow> bool) ::
+    (('a \<times> bool list) list \<times> _) list \<times> _ \<Rightarrow> bool"
+  and step_invariant = "rexp_DA.step_invariant (\<sigma> \<Sigma>) (\<lambda>a r. pnorm_dual (Co\<DD> \<Sigma> a r)) id n"
+  and closure_invariant = "rexp_DA.closure_invariant (\<sigma> \<Sigma>) (\<lambda>a r. pnorm_dual (Co\<DD> \<Sigma> a r)) final_dual id n"
+  and counterexampleRE = "rexp_DA.counterexample (\<sigma> \<Sigma>) (\<lambda>x. pnorm_dual (rexp_dual_of (inorm x))) (\<lambda>a r. pnorm_dual (Co\<DD> \<Sigma> a r)) final_dual id n"
+  and reachable = "rexp_DA.reachable (\<sigma> \<Sigma>) (\<lambda>x. pnorm_dual (rexp_dual_of (inorm x))) (\<lambda>a r. pnorm_dual (Co\<DD> \<Sigma> a r)) id n"
+  and automaton = "rexp_DA.automaton (\<sigma> \<Sigma>) (\<lambda>x. pnorm_dual (rexp_dual_of (inorm x))) (\<lambda>a r. pnorm_dual (Co\<DD> \<Sigma> a r)) id n"
+  by unfold_locales (auto simp only: comp_apply id_apply
+    wf_inorm lang_inorm
+    wf_dual_pnorm_dual lang_dual_pnorm_dual
+    wf_dual_rexp_dual_of lang_dual_rexp_dual_of
+    wf_dual_lderiv_dual lang_dual_lderiv_dual
+    lang_dual_final_dual dest!: lang_dual_subset_lists)
 
 definition check_eqv where
 "check_eqv n \<phi> \<psi> \<longleftrightarrow> wf_formula n (FOr \<phi> \<psi>) \<and>
